
The Fourier Transform, Fourier Series, Laplace transform and Z-transform  are included 

---
The virtues of employing an input of the form $Ae^{i\omega t}$  are : 
1. Compactness of notation  --> $\alpha cos(\omega t + \phi) + \beta sin(\omega t +  \psi)$ can be represented  by $Re(Ae^{i\omega t})$
2. The fact that the differentiation of the above (sinusoids) function amounts to multiplication by $i\omega$  -> replacing calculus by algebra
3. The fact the steady-state response of the system to the input will have the form of $e^{i\omega t}$

### 8.1 Fourier Series(Finite Fourier Transform)
#### Fourier Series
For a decomposition of the $F(t)$, 
$$\omega_n = \frac{2\pi n}{L}$$
[[8. The transforms of Applied Mathmatics 2023-01-09 19.04.40.excalidraw|proof of the Fourier Series]]

then we have the Fourier Series: 
$$
F(t) = \sum^{\infty}_{-\infty} c_n e^{i n t} \tag{13}
$$
where
$$c_m = \frac{1}{2\pi} \int^{\pi}_{-\pi}F(t) e^{imt} dt \tag{14}$$
valid whenever the series above is uniformly convergent

**Definition : if F has period $2\pi$ and is integrable over $[-\pi, \pi]$, the  series with coefficients above is  called the Fourier Series for $F$ , and the numbers $c_n$ are called the Fourier  coefficients of $F$**

more generally, if $F$ has a period of $L$, then: 
$$F(t) = \sum^{\infty}_{-\infty} c_n e^{-i n\frac{2\pi t}{L}}$$
where
$$c_n = \frac{1}{L} \int^{L/2}_{-L/2} F(t) e^{-i n \frac{2\pi t}{L}} dt$$
then  we  introduce: 
$$F(t) =: f(e^{it})$$
and we can derive the equation of the Fourier transform from the following steps:
[[8. The transforms of Applied Mathmatics 2023-01-09 20.22.54.excalidraw|the derivation of the relationship with Laurent Series]]

#### the Poisson Formula(????)
we want to  solve the Dirichlet problem for the unit disk and $U(\theta)$ has a Fourier expansion: 
$$U(\theta) = \sum^{\infty}_{n = -\infty}\left[ \frac{1}{2 \pi} \int^{\pi}_{-\pi} U(\phi) e^{-in\phi} d\phi\right] e^{in\phi}$$
where we insert 
$$c_m = \frac{1}{2\pi}\int^{\pi}_{-\pi} F(t) e^{-imt} dt$$
thus
$$U(\theta) = \frac{1}{2\pi} \int^{\infty}_{-\infty} U(\phi) d\phi + 2\sum^{\infty}_{n = 1} \frac{1}{2\pi} \int^{\infty}_{-\infty} U(\phi)\cos n(\theta - \phi) d\phi$$
Now we we a device known as Abel-Poisson summation to sum the series and we have: 
$$g(r,\theta) := \frac{1}{2\pi} \int^{\infty}_{-\infty} U(\phi) d\phi + \frac{1}{\pi}\sum^{\infty}_{n = 1} \int^{\infty}_{-\infty} U(\phi) r^n \cos n(\theta - \phi) d\phi$$
with the equality
$$1 + 2\sum^{\infty}_{n=1} r^n\cos n(\theta -\phi) = \frac{ 1 - r^2}{1 - 2r \cos(\theta -\phi) + r^2}$$
we can finally arrive the Poisson formula: 
the Poisson formula ( the detailed derivation can be referenced from the textbook p451)
$$u\left(re^{i\theta}\right) = \frac{1 - r^2}{2 \pi} \int^{\pi}_{-\pi} \frac{U(\phi)}{1 - 2r\cos(\theta - \phi) + r^2} d\phi$$

#### Relevant Theorems
**Theorem 1. If the integral  $\int^{\pi}_{-\pi}|F(t)|^2$ exists, then the Fourier series defined by the above equations exists and it  converges to F in the mean square sense**
$$\lim_{N\to \infty} \int^{\pi}_{-\pi} \left| F(t) - \sum^{N}_{n = -N} c_n e^{int}  \right|^2 dt  = 0$$
**Theorem 2. Suppose that $F$ is Periodic and Piecewise smooth, then the Fourier Series For the converges to $\frac{1}{2}[F(\tau_{j+} + F(\tau_{j-})]$ at the point of discontinuity**

**Theorem 3. Suppose the Fourier expansion is valid and the derived series converges on $[-\pi, \pi]$ Then**
$$\sum^{\infty}_{n = -\infty} inc_n e^{int} = \frac{d}{dt}\sum^{\infty}_{n = -\infty} c_n e^{int}$$

#### Fourier Transform and Fourier analysis
Suppose that F has a convergent Fourier series expansion:
[[8. The transforms of Applied Mathmatics 2023-01-10 12.38.47.excalidraw|brief solution of the sin\theta]]

### 8.2 The Fourier transform
We move on to the decomposing arbitrary functions into sinusoids, 
we firstly assume that we are given a nonperiodic function $F(t)$, and $-\infty< t < \infty$, and continuously differentiable. Then if we pick an interval of the form $(-\frac{L}{2}, \frac{L}{2})$,we can represent $F(t)$ by 
$$F(t) =  \sum^{\infty}_{n = -\infty} c_n e^{in \frac{2\pi t}{L}}, \qquad  -\frac{L}{2} < t < \frac{L}{2}$$
where 
$$c_n = \frac{1}{L} \int^{\frac{L}{2}}_{-\frac{L}{2}} F(t) e^{in\frac{-2\pi t}{L}} dt$$
so when $L \to \infty$
we define 
$$g_n = \frac{c_nL}{2\pi} = \frac{1}{2\pi}\int^{\frac{L}{2}}_{-\frac{L}{2}} F(t) e^{-in\frac{2\pi t}{L}} dt$$since we use the $n^{th}$ L in the function,  we introduce the factor $[(n+1)-n]\equiv 1$ into the equation, and
$$F_L(t) = \sum^{\infty}_{-\infty} g_n e^{in \frac{2\pi t}{L}} \frac{2\pi  [(n+1) - n]}{L}$$
so we rewrite the $\omega_n = \frac{n 2\pi}{L}$, producing: 
$$F_L(t) = \sum^{\infty}_{n = -\infty} G_L(\omega_n) e^{i\omega_n t}(\omega_{n+1} - \omega_n) \tag{5}$$
and
$$G_L(\omega) := \frac{1}{2\pi} \int^{\frac{L}{2}}_{-\frac{L}{2}} F(t) e^{-i\omega t} dt$$
so we define
$$\boxed{G_L(\omega) := \frac{1}{2\pi} \int^{\frac{L}{2}}_{-\frac{L}{2}} F(t) e^{-i\omega t} dt} $$
as  the *Fourier Transform* of $F$, and the $F(t)$ become a Riemann sum: 
$$ \boxed{ F(t) = \int^{\infty}_{-\infty}G(\omega) e^{i\omega t}d\omega}$$
called the *Fourier inverse Formula* of $G(\omega)$
the two equations above are the essence of Fourier transform theory.

**Theorem 4. Suppose that $F(t)$ is piecewise on every bounded interval and $\int^{\infty}_{-\infty}|F(t)|dt$ exists, Then the Fourier transform $G(\omega)$, of $F$ exists and**
$$\text{p.v.} \int^{\infty}_{-\infty} G(\omega) e^{i\omega t} dt = \begin{cases}
F(t) \qquad \qquad \quad \text{where F is continuous} \\
\frac{F(t+) + F(t-)}{2} \qquad \text{otherwise}
\end{cases}$$
where $p.v.$ means the present value

the example can be found in the page 481

### 8.3 The Laplace transform

In the previous section is used for solve  a linear system by means of frequency analysis, The strategy we were employing can be stated -> if the linear system is forced by a sinusoid input function, $e^{i\omega t}$, and then we expect  that there ought to be a solution of the form $Ae^{i\omega t}$, which is a solution of the same frequency.

but Now this may not be the only solution, for example, consider the problem of finding a function $f(t)$ that satisfies the equation: 
$$\frac{d^2 f(t)}{dt^2} + 2\frac{df(t)}{dt} + f(t) = e^{i 2 t}$$
It has the solution of $Ae^{i2t}$ with $A = \frac{1}{4i-3}$ , but considering the solution of the associated homogenous equation $f(t)$
$$\frac{d^2 f(t)}{dt^2} + 2\frac{df(t)}{dt} + f(t) = 0$$
the function f(t) can be added to the solution of the eq above

like -> the function
$$\frac{1}{4i - 3}e^{i2t} + 7e^{-t}$$ is also one of the solution of  the equation, and $7e^{-t}$ is a "homogenous solution"

Note that for most physical systems, these homogenous solutions are ==transient== in nature. (that is, the homogenous part die out as time increases like $e^{-t}$) -> the reason is that for the most physical systems. If not forced, is eventually come to rest due to dissipative phenomena. -> called *asymptotically stable*

we should consider the system may  start in some "initial configuration" at t=0 that probably doesn't coincide with steady-state solution, and also, the inputs at "t=0" doesn't drive the system for all $t\geq 0$
the Laplace transform handles both of the problem above 

for the input function, $F(t)$ is defined for all $t\geq 0$, so we set $F(t) =0$ for t< 0, and then consider the Fourier transform of $F$
$$G(\omega) = \frac{1}{2\pi} \int^{\infty}_{-\infty} F(t) e^{-i\omega t} dt$$
since $F(t) = 0(t\leq 0)$, we have:
$$G(\omega) = \frac{1}{2\pi} \int^{\infty}_{0} F(t) e^{-i\omega t} dt \tag{3}$$
we have that $F$ is sufficiently well behaved near infinity(we shouldn't be precise)-> the equation (3) above defines a function of $\omega$ that is ==analytic in the lower-half-plane== $Im(\omega)< 0$,  and the derivation of the frequency omega is given by: 
$$\frac{dG(\omega)}{d\omega} = \frac{-i}{2\pi} \int^{\infty}_{0}tF(t) e^{-i\omega t} dt$$
and the lower half-plane is appropriate because (since $|e^{i\theta t}| =1$)
$$\left|e^{-i\omega t}\right| = e^{(\text{Im}\omega )t}$$
is bounded there, and If we let $\omega$ be pure imaginary say $\Large\omega = -is$ with nonnegative, we create 
$$g(s) := 2\pi G(-is)$$
and we reach a function
$$\boxed{g(s) = \int^{\infty}_{0}F(t) e^{-st} dt \tag{5}}$$
this is called the *Laplace Transform* of $F(t)$
and It's often useful to indicate the relation between $g(s)$  and $F(t)$ by employing this notation: 
$$g(s) = \mathcal{L}\{F\}(s)$$
for example: [[8. The transforms of Applied Mathmatics 2023-01-10 18.04.12.excalidraw|simple example]]
Remark that the F(t) the integral in the Eq above may converge  even if F doesn't approach zero as $t \to \infty$ , provided $s$ is sufficiently large, for example the function $F(t) = e^{7t}$->  $\frac{e^{(7-s)b} - 1}{7-s}$, then  the s should be large when the s>7, the function converges to  $(s -7)^{-1}$ as $b \to \infty$

Accordingly, we should say  that the equation (5) defines the Laplace transform for any complex value of $s$ for which the integral converges. In essence the Laplace transform is able to encompass more function than the Fourier transform. 

for a simple extension of the preceding computation, By interpreting the statement with various choice of the constant $a$Ôºåwe are able to derive the Laplace transform table
[[üìòClassNotes/üìêMathmatics/‚ÑπÔ∏èComplex Variables/Ë°•ÂÖÖÂÜÖÂÆπ/Â∏∏Áî®ÊãâÊôÆÊãâÊñØÂèòÊç¢Ë°®]]
also there are some important relationships:
$$\mathcal{L}\{F(t)e^{-at}\}(s) =  \mathcal{L}\{F\}(s+a)$$

Now if $F'$ is sufficiently well behaved so that integration by parts is permitted, this becomes: 
$$\mathcal{L}\{F'\}(s) = \int^{\infty}_{0}e^{-st}F'(t)dt =  \left. e^{-st} F(t)\right|^{\infty}_0 + \int^{\infty}_{0} se^{-st}F(t)dt$$
thus
$$\boxed{\mathcal{L}\{F'\}(s) = s\mathcal{L}\{F\}(s)-F(0)}$$
also, the Iteration of the equation results in
$$L\{F''\}(s) = s\mathcal{L}\{F'\}(s) - F'(0) = s^2\mathcal{L}\{F\}(s) - sF(0) - F'(0)$$
and in general 
$$\mathcal{L}\{F^{(k)}\}(s) = s^k \mathcal{L}\{F\}(s) - s^{k-1} F(0) - s^{k-2} F'(0) - ... - F^{(k-1)}(0) \tag{8}$$

**Theorem 5. Suppose that the function F(t) and it's first n-1 derivatives are continuous for $t\geq 0$ ,  and that $F^{(n)}(t)$ is piecewise smooth on every finite interval $[0,b]$, Also suppose that there are positive constants M, $\alpha$ such that for k=0,1,2,....n-1**
$$\left|F^{(k)}(t)\right|\leq Me^{\alpha t} \qquad (t\geq 0)$$
**Then  the Laplace transforms of $F, F', ...$. exists for Re(s)>$\alpha$ and Eq(8) is valid for k= 1,2,...n**

**Theorem 6. Suppose  that F(t) is piecewise smooth on every finite interval $[0,b]$ and $|F(t)|$ is bounded by $Me^{at}$ for  $t\geq 0$ , Then the $\mathcal{L}\{F\}(s)$ exists for $Re(s)>\alpha$. and for all $t>0$ and $a>\alpha$**
$$\frac{F(t+) + F(t-)}{2} = \frac{1}{2\pi i} p.v.\int^{a + i\infty}_{a - i\infty}\mathcal{L}\{F\}(s) e^{st} ds$$


### 8.4 The z-transform
often in Practice we encounter the function that are discrete data structures. For example, when a continuous 

so we denote a discrete sequence of numbers by $a_n$ we assume n to take integer values from $-\infty$ to $\infty$ we also allow the $a_n$  can be complex, As examples consider: 
$$\{a\} \to ...\frac{1}{16}, \frac{1}{8}, \frac{1}{4}, \frac{1}{2}, 1,\frac{1}{2},\frac{1}{4},.....$$
for sample $2^{-|x|}$ at integers  x=n 
$$\{a\} = -1,1,-1,1,.....$$
for sample $cos(\pi x)$
the z-transform of the sequence of the sequence $a(n)$ is defined as the sum of the series 
$$\boxed{A(z) := \sum^{\infty}_{n = -\infty} a_n z^{-n}}$$
$$A(z)= ...+ A(-2)z^{2} + A(-1)z^{1} + A(0) + A(1) z^{-1}+ ....$$

Theorem 7. **Let A(z) be the z-transform of the sequence  $[a(n): -\infty <n < \infty$ in the annulus $a < |z| < b$, Then**
$$a_n = \frac{1}{2\pi i} \oint_\Gamma A(\zeta) \zeta^{n-1}d\zeta \qquad (n =0, \pm 1, \pm 2,....)$$
**where $\Gamma$ is any positively oriented simple closed contour lying in the annulus and encircling the origin**


Theorem 8. **Let A(z) be the z-transform of the sequence  $[a(n): -\infty <n < \infty$ in the annulus $a < |z| < b$, Then the corresponding z-transform of the shifted sequence $\{b(n) = a(n+1): -\infty < n < \infty\}$ is given by $zA(z)$, and also , the $c(n) = a(n+N)$ is given by $z^NA(z)$ for any positive N**

r


