$$\large\begin{cases}
\sin \alpha + \sin \beta = 2 \sin(\frac{\alpha +\beta}{2})\cos(\frac{\alpha - \beta}{2}) \\
\sin \alpha - \sin \beta = 2 \cos(\frac{\alpha +\beta}{2})\sin(\frac{\alpha - \beta}{2}) \\
\cos \alpha + \cos \beta = 2 \cos (\frac{\alpha + \beta}{2}) \cos(\frac{\alpha - \beta}{2}) \\
\cos \alpha - \cos \beta = -2 \sin ({\frac{\alpha +\beta}{2}}) \sin(\frac{\alpha -\beta}{2})
\end{cases}$$
$$\large\begin{cases}
\sin \alpha \sin \beta = -\frac{1}{2} [\cos(\alpha + \beta) - \cos(\alpha - \beta)] \\
\cos \alpha \cos \beta = \frac{1}{2}[\cos(\alpha + \beta) + \cos(\alpha -\beta)] \\ 
\sin\alpha \cos\beta = \frac{1}{2}[\sin(\alpha + \beta) + \sin(\alpha -\beta)] \\
\cos\alpha \sin \beta = \frac{1}{2} [\sin(\alpha + \beta) - \sin(\alpha -\beta)]
\end{cases}$$
