根据 : 
$$\cos 2 \theta =  2 \cos^{2} \theta - 1 = 1 - 2 \sin ^{2} \theta$$
可以得到如下公式 : 
$$\sin^{3} \omega t =  \frac{3}{4} \sin  \omega t  + \frac{1}{4} \sin 3 \omega t \approx   \frac{3}{4} \sin \omega t$$
$$\sin^{2} \omega t \cos \omega t  = \frac{1}{4} \cos \omega t  - \frac{1}{4} \cos 3 \omega t \approx  \frac{1}{4}  \cos \omega t$$
$$\sin \omega t  \cos^{2} \omega t = \frac{1}{4}  \sin \omega t + \frac{1}{4} \sin 3\omega t \approx \frac{1}{4} \sin \omega t$$
$$\cos^{3} \omega t  = \frac{3}{4} \cos \omega t +  \frac{1}{4}   \cos 3 \omega  t \approx \frac{3}{4} \cos \omega t$$
