$$\begin{equation}
\begin{cases}
(x^2 + 5) \frac{du}{dx} - 2\frac{d^2u}{dx^2} = 2x  , \qquad x \leq 0 \leq 1\\
u = 5 , \qquad \qquad  x = 0 \\
2 \frac{du}{dx}  = x + 3 \qquad x = 1
\end{cases}
\end{equation}$$

---
积分并约去$\delta u_j$，得到：
$$\int_{0}^{1} (x^2 + 5) \frac{d \Phi_i}{dx} \Phi_j u_i dx + 2 \int_{0}^{1}\frac{d\Phi_i}{dx}\frac{d\Phi_j}{dx} u_i dx = \int_{0}^{1} 2x \Phi_j dx + \left. \left( 2\frac{d u}{dx} \Phi_j\right) \right|_0^1$$
代入可得 : 
$$\int_{0}^{1} (x^2 + 5) \frac{d \Phi_i}{dx} \Phi_j u_i dx + 2 \int_{0}^{1}\frac{d\Phi_i}{dx}\frac{d\Phi_j}{dx} u_i dx = \int_{0}^{1} 2x \Phi_j dx + \left. \left[ (x+ 3)\Phi_j\right] \right|_0^1$$


$$\int_{0}^{1} (x^2 + 5) \frac{d \Phi_i}{dx} \Phi_j u_i dx + 2 \int_{0}^{1}\frac{d\Phi_i}{dx}\frac{d\Phi_j}{dx} u_i dx = \int_{0}^{1} 2x \Phi_j dx + 4\Phi_j(1) - 3\Phi_j(0)$$

其中，我们取
$$\int_{0}^{1} \left[ 2\frac{d\Phi_i}{dx} \frac{d\Phi_j}{dx} dx +  (x^2 + 5) \frac{d\Phi_i}{dx}\Phi_j\right] dx= A_{ij}$$
